src/Prelude_proof.thy
@@ -1,0 +1,8 @@
+theory Prelude_proof imports Prelude begin
+
+(* FIXME move to lib_proof *)
+lemma set_butlast_lessThan:"set (butlast [0..<n]) = {0..<n -1}"
+apply (case_tac n,force+)
+done
+
+end
